Communication_Topology_Soundness.thy
@@ -7,16 +7,39 @@ theory Communication_Topology_Soundness
 begin
 
 
+lemma xyz: "
+  \<lbrakk> 
+    (\<V>, \<C>) \<Turnstile>\<^sub>e e;
+    [[] \<mapsto> \<langle>e;Map.empty;[]\<rangle>] \<rightarrow>* \<E>'
+  \<rbrakk> \<Longrightarrow>
+  (\<forall> \<pi> . \<E>' \<pi> = Some (\<langle>e'; \<rho>'; \<kappa>'\<rangle>) \<longrightarrow> \<parallel>\<rho>'\<parallel> \<sqsubseteq> \<V>)
+"
+ apply (rule allI, rule impI)
+ apply (drule flow_sound[of \<V> \<C> e \<E>' _ e' \<rho>' \<kappa>'], auto)
+done
 
+
+lemma topology_one_shot_sound: "
+  [[] \<mapsto> \<langle>e;Map.empty;[]\<rangle>] \<rightarrow>* \<E>' \<Longrightarrow> (\<V>, \<C>) \<Turnstile>\<^sub>e e \<Longrightarrow> 
+  one_max (abstract_send_paths \<V> x e) \<Longrightarrow> 
+  \<E>' \<pi> = Some (\<langle>LET x = CHAN \<lparr>\<rparr> in e';\<rho>';\<kappa>'\<rangle>) \<Longrightarrow> 
+  one_shot \<E>' (Ch \<pi> x)
+"
+ apply (drule xyz, auto)
+ apply (simp add: one_shot_def send_paths_def abstract_value_env_precision_def env_to_abstract_value_env_def)
+ apply (simp add: one_max_def abstract_send_paths_def control_paths_def abstract_send_sites_def)
+sorry
 
 theorem topology_pair_sound : "
   \<lbrakk>
-    (x, t) \<TTurnstile> e; 
+    (x, t) \<TTurnstile> e;
     [[] \<mapsto> \<langle>e; empty; []\<rangle>] \<rightarrow>* \<E>'
   \<rbrakk> \<Longrightarrow>
-  \<langle>\<langle>\<E>' ; x\<rangle>\<rangle> \<preceq> t
+  \<langle>\<langle>\<E>'; x\<rangle>\<rangle> \<preceq> t
 "
+ apply (erule topo_pair_accept.cases; auto)
 sorry
+
 
 lemma topology_sound': "
   (x, \<A> x) \<TTurnstile> e \<Longrightarrow> [[] \<mapsto> \<langle>e; Map.empty; []\<rangle>] \<rightarrow>* \<E>' \<Longrightarrow> (\<langle>\<langle>\<E>'\<rangle>\<rangle>) x \<preceq> \<A> x
@@ -28,7 +51,7 @@ done
 
 theorem topology_sound : "
   \<lbrakk>
-    \<A> \<bind> e; 
+    \<A> \<bind> e;
     [[] \<mapsto> \<langle>e; empty; []\<rangle>] \<rightarrow>* \<E>'
   \<rbrakk> \<Longrightarrow>
   \<langle>\<langle>\<E>'\<rangle>\<rangle> \<sqsubseteq>\<^sub>t \<A>
